Cleaned up proofs for Rocq; Replaced full AMM

tests/hevm/pass/multisource/amm/amm.sol
@@ -1,39 +1,138 @@
 pragma solidity >=0.8.0;
 
-interface Token {
-  function balanceOf(address) external view returns (uint256);
-  function transferFrom(address from, address to, uint256 value) external returns (uint);
+contract Token {
+    uint256 public totalSupply;
+    mapping (address => uint256) public balanceOf;
+    mapping (address => mapping (address => uint256)) public allowance;
+
+    constructor(uint256 _totalSupply) {
+        totalSupply = _totalSupply;
+        balanceOf[msg.sender] = _totalSupply;
+    }
+
+
+    function approve(address spender, uint256 value) public returns (bool) {
+        if(spender != msg.sender) {
+            allowance[msg.sender][spender] = value;
+        }
+        return true;
+    }
+
+    function transfer(uint256 value, address to) public returns (bool) {
+        balanceOf[msg.sender] = balanceOf[msg.sender] - value;
+        balanceOf[to] = balanceOf[to] + value;
+        return true;
+    }
+
+    function transferFrom(address from, address to, uint256 value) public returns (bool) {
+        if(from != msg.sender && allowance[from][msg.sender] != type(uint256).max) {
+            allowance[from][msg.sender] = allowance[from][msg.sender] - value;
+        }
+        balanceOf[from] = balanceOf[from] - value;
+        balanceOf[to] = balanceOf[to] + value;
+        return true;
+    }
 }
 
-contract Amm {
 
+contract Amm is Token {
+    uint256 internal constant MINIMUM_LIQUIDITY = 1000;
     Token token0;
     Token token1;
+    uint256 reserve0;
+    uint256 reserve1;
 
-    constructor(address t0, address t1) {
+    constructor(address t0, address t1, uint256 liquidity) Token(liquidity - MINIMUM_LIQUIDITY) {
         require (t0 != t1);
         token0 = Token(t0);
         token1 = Token(t1);
+
+        require(liquidity*liquidity == token0.balanceOf(address(this)) * token1.balanceOf(address(this)), "Invalid initial liquidity");
+        require(liquidity > 0, 'Invalid initial liquidity');
+        totalSupply = liquidity;
+        balanceOf[address(this)] =  MINIMUM_LIQUIDITY;
+        balanceOf[msg.sender] = liquidity - MINIMUM_LIQUIDITY;
+        reserve0 = token0.balanceOf(address(this));
+        reserve1 = token1.balanceOf(address(this));
     }
 
-    function swap0(uint256 amt) public returns (uint) {
-        uint256 reserve0 = token0.balanceOf(address(this));
-        uint256 reserve1 = token1.balanceOf(address(this));
+    function mint(address to) public returns (uint256 liquidity) {
+      require(totalSupply != 0);
 
-        token0.transferFrom(msg.sender, address(this), amt);
-        token1.transferFrom(address(this), msg.sender, (reserve1*amt)/(reserve0+amt));
+      uint256 balance0 = token0.balanceOf(address(this));
+      uint256 balance1 = token1.balanceOf(address(this));
 
-        return 1;
+      uint256 amount0 = balance0 - reserve0;
+      uint256 amount1 = balance1 - reserve1;
+
+      uint256 liq0 = amount0 * totalSupply / reserve0;
+      uint256 liq1 = amount1 * totalSupply / reserve1;
+
+      if (liq0 <= liq1) {
+        liquidity = liq0;
+      } else {
+        liquidity = liq1;
+      }
+
+      require(liquidity != 0, "Insufficient liquidity");
+      totalSupply += liquidity;
+      balanceOf[to] += liquidity;
+
+      reserve0 = balance0;
+      reserve1 = balance1;
     }
 
-    function swap1(uint256 amt) public returns (uint) {
-        uint256 reserve0 = token0.balanceOf(address(this));
-        uint256 reserve1 = token1.balanceOf(address(this));
+    function burn(uint256 liquidity, address to) public {
+      require(totalSupply != 0);
 
-        token1.transferFrom(msg.sender, address(this), amt);
-        token0.transferFrom(address(this), msg.sender, (reserve0*amt)/(reserve1+amt));
+      uint256 amount0 = (liquidity * reserve0) / totalSupply;
+      uint256 amount1 = (liquidity * reserve1) / totalSupply;
 
-        return 1;
+      totalSupply -= liquidity;
+      balanceOf[msg.sender] -= liquidity;
+
+      token0.transfer(amount0, to);
+      token1.transfer(amount1, to);
+
+      reserve0 = token0.balanceOf(address(this));
+      reserve1 = token1.balanceOf(address(this));
     }
 
+    function swap0(uint256 amount1Out, address to) public {
+      require(amount1Out > 0, 'Insufficient output amount');
+      require(amount1Out < reserve1, 'Insufficient liquidity');
+      require(to != address(token0) && to != address(token1), 'Invalid TO');
+
+      token1.transfer(amount1Out, to);
+
+      uint256 balance0 = token0.balanceOf(address(this));
+      uint256 balance1 = token1.balanceOf(address(this));
+
+      require(balance0 > reserve0, 'Insufficient input amount');
+      uint256 amount0In = balance0 - reserve0;
+
+      require(amount1Out <= (reserve1 * amount0In / (reserve0 + amount0In)), 'K');
+
+      reserve0 = balance0;
+      reserve1 = balance1;
+    }
+
+    function swap1(uint256 amount0Out, address to) public {
+      require(amount0Out > 0, 'Insufficient output amount');
+      require(amount0Out < reserve0, 'Insufficient liquidity');
+      require(to != address(token0) && to != address(token1), 'Invalid TO');
+
+      token0.transfer(amount0Out, to);
+
+      uint256 balance0 = token0.balanceOf(address(this));
+      uint256 balance1 = token1.balanceOf(address(this));
+
+      require(balance1 > reserve1, 'Insufficient input amount');
+      uint256 amount1In = balance1 - reserve1;
+
+      require(amount0Out <= (reserve0 * amount1In / (reserve1 + amount1In)), 'K');
+
+      reserve0 = balance0;
+      reserve1 = balance1;
+    }
 }
