tests/rocq/amm/Theory.v
@@ -1,4 +1,5 @@
 Require Import Stdlib.ZArith.ZArith.
+Require Import Stdlib.ZArith.Zmin.
 Require Import ActLib.ActLib.
 Require Stdlib.Strings.String.
 From Stdlib Require Import Lia.
@@ -10,19 +11,14 @@ Import Amm.
 
 Definition MAX_ADDRESS := UINT_MAX 160.
 
-Ltac convert_neq :=
-  repeat match goal with
-    [ H : _ <> _ |- _ ] => let H_og := fresh H "'" in eapply not_eq_sym in H as H_og; eapply Z.eqb_neq in H; eapply Z.eqb_neq in H_og
-  end.
-
-Ltac convert_eq :=
-  repeat match goal with
-    [ H : _ = _ |- _ ] => let H_og := fresh H "'" in eapply eq_sym in H as H_og; eapply Z.eqb_eq in H; eapply Z.eqb_eq in H_og
-  end.
-
 Ltac destructAnds :=
   repeat match goal with
     [ H : _ /\ _ |- _ ] => destruct H
+  end.
+
+Ltac convert_neq :=
+  repeat match goal with
+    [ H : _ <> _ |- _ ] => eapply not_eq_sym in H; eapply Z.eqb_neq in H
   end.
 
 Ltac rewrite_eqs :=
@@ -30,20 +26,79 @@ Ltac rewrite_eqs :=
     [ H : _ =? _ = _ |- _ ] => rewrite H
   end.
 
+
+  Ltac rewrite_eqbs :=
+  repeat match goal with
+  | [ H : ?a = ?b |- context [?a =? ?b] ] =>
+    rewrite (proj2 (Z.eqb_eq a b) H)
+  | [ H : ?a = ?b |- context [?b =? ?a] ] =>
+    rewrite (proj2 (Z.eqb_eq b a) (eq_sym H))
+  | [ H : ?a <> ?b |- context [?a =? ?b] ] =>
+    rewrite (proj2 (Z.eqb_neq a b) H)
+  | [ H : ?a <> ?b |- context [?b =? ?a] ] =>
+    rewrite (proj2 (Z.eqb_neq b a) (not_eq_sym H))
+  end.
+
+Ltac rewrite_b_right H :=
+  match goal with
+  | [ H : _ =? _ = true |- _ ] => apply Z.eqb_eq in H as H'; rewrite <- H' in * 
+    end.
+
+Ltac rewrite_b_left H :=
+  match goal with
+  | [ H : _ =? _ = true |- _ ] => apply Z.eqb_eq in H as H'; rewrite H' in *
+    end.
+
+Ltac bool_to_prop :=
+  repeat match goal with
+  | [ H : (_ =? _)%Z = true  |- _ ] => apply Z.eqb_eq in H
+  | [ H : (_ =? _)%Z = false |- _ ] => apply Z.eqb_neq in H
+  | [ H : (_ <? _)%Z = true  |- _ ] => apply Z.ltb_lt in H
+  | [ H : (_ <? _)%Z = false |- _ ] => apply Z.ltb_ge in H
+  | [ H : (_ <=? _)%Z = true  |- _ ] => apply Z.leb_le in H
+  | [ H : (_ <=? _)%Z = false |- _ ] => apply Z.leb_gt in H
+  | [ H : (_ >? _)%Z = true  |- _ ] => apply Z.gtb_lt in H
+  | [ H : (_ >? _)%Z = false |- _ ] => apply Z.gtb_ltb in H
+  | [ H : (_ >=? _)%Z = true  |- _ ] => apply Z.geb_le in H
+  | [ H : (_ >=? _)%Z = false |- _ ] => apply Z.geb_leb in H
+  end.
+
+Ltac prop_to_bool :=
+  repeat match goal with
+  | [ H : @eq Z _ _        |- _ ] => apply Z.eqb_eq in H
+  | [ H : _ <> _           |- _ ] => apply Z.eqb_neq in H
+  | [ H : Z.lt _ _         |- _ ] => apply Z.ltb_lt in H
+  | [ H : _ > _            |- _ ] => apply Z.le_antisymm
+  | [ H : Z.le _ _         |- _ ] => apply Z.leb_le in H
+  | [ H : Z.gt _ _         |- _ ] => apply Z.gtb_lt in H
+  | [ H : Z.ge _ _         |- _ ] => apply Z.geb_le in H
+  end.
+
+Ltac destruct_ifs :=
+  repeat match goal with
+  | [ |- context [if ?a =? ?b then _ else _] ] =>
+    destruct (a =? b) eqn:?; bool_to_prop
+  | [ H : context [if ?a =? ?b then _ else _] |- _ ] =>
+    destruct (a =? b) eqn:?; bool_to_prop
+  end.
+
+
+
+
 Lemma le_neq_lt : forall n : Z, 0 <= n -> n <> 0 -> 0 < n.
 Proof.
   lia.
 Qed.
 
 Lemma div_prop:
-     forall a b c,
+     forall (a b c : Z),
      0 <= b
   -> 0 <= c
   -> 0 < a + c
   -> a * b <= (a + c) * (b - b * c / (a + c)).
 Proof.
   intros a b c HbNonneg HcNonneg HacPos.
-  rewrite Z.mul_sub_distr_l.
+  rewrite Z.mul_sub_distr_l with (n :=a + c) (m := b).
   rewrite Z.mul_comm with (n := a + c) (m := b).
   rewrite Z.mul_add_distr_l.
   rewrite Z.mul_comm with (n := a) (m := b).
@@ -114,59 +169,1030 @@ Proof.
   - lia.
 Qed.
 
-Lemma swap0_post0_witness : swap0_post0.
+  
+Lemma ERC20_allowance_zero :
+  forall (Before : address) (ENV : Env) (T : Token.State) (a : address),
+    Token.reachableBefore Before T
+  -> Before <= a
+  -> forall i, Token.allowance T a i = 0.
 Proof.
-  intros NA NA' ENV STATE STATE' amt HConds Hreach Htransition.
-  destruct HConds.
-  destruct Htransition; simpl.
-  - destructAnds. convert_neq. rewrite_eqs.
-    rewrite Z.eqb_refl.
-    apply div_prop; lia.
-  - destructAnds. convert_neq. rewrite_eqs.
-    rewrite Z.eqb_refl.
-    apply div_prop; lia.
-  - reflexivity.
+  intros Before ENV T a HreachBefore.
+  destruct HreachBefore as [T_Init [HinitBefore HmultiBefore]].
+  apply step_multi_step 
+  with (P := fun s s' => (Before <= a -> forall i : address, Token.allowance s a i = 0) -> 
+                         Before <= a -> forall i : address, Token.allowance s' a i = 0) in HmultiBefore.
+    - destruct HinitBefore as [? ? ? ? Hinit H_leq_before].
+      apply HmultiBefore.
+      destruct Hinit. destruct H_conds; simpl; reflexivity.
+    - intros s s' HstepBefore HzeroS.
+      destruct HstepBefore as [ENV' [NextAddr [NextAddr' [H_transition H_NextAddr_leq_before]]]].
+      destruct H_transition; destruct H;
+        try (destruct H; assumption).
+      + (* transferFrom *)
+        destruct H; simpl; try assumption.
+        * destruct (a =? src) eqn:H_a_eq_src.
+          -- apply Z.eqb_eq in H_a_eq_src. rewrite <- H_a_eq_src. intros.
+            assert (Token.allowance s a (Caller ENV') = 0). auto.
+            assert (Caller ENV' <> src) as H_caller_neq_src. { destructAnds. assumption. }
+            destruct H_conds. apply H_iff3 in H_caller_neq_src. 
+            assert (amount = 0). { apply Z.le_antisymm; try lia.
+              rewrite <- H_a_eq_src in H_caller_neq_src. rewrite H0 in H_caller_neq_src. lia.
+            }
+            destruct (i =? Caller ENV'); try lia; auto.
+          -- assumption.
+        * destruct (a =? src) eqn:H_a_eq_src.
+          -- apply Z.eqb_eq in H_a_eq_src. rewrite <- H_a_eq_src. intros.
+            assert (Token.allowance s a (Caller ENV') = 0); auto.
+            assert (Caller ENV' <> src) as H_caller_neq_src. { destructAnds. assumption. }
+            destruct H_conds. apply H_iff3 in H_caller_neq_src. 
+            assert (amount = 0). { apply Z.le_antisymm; try lia.
+              rewrite <- H_a_eq_src in H_caller_neq_src. rewrite H0 in H_caller_neq_src. lia.
+            }
+            destruct (i =? Caller ENV'); try lia; auto.
+          -- assumption.
+      + (* approve *)
+        destruct H; simpl; try assumption.
+        * destruct H_conds; auto.
+          intro H_NA_leq_x.
+          assert (Caller ENV' < a). {
+            apply Z.lt_le_trans with (m := NextAddr).
+            * assumption.
+            * lia.
+          }
+          assert (a =? Caller ENV' = false). simpl. lia.
+          rewrite_eqs.
+          apply HzeroS. assumption.
+      + (* burnFrom *)
+        destruct H; simpl; try assumption.
+        * destruct (a =? src) eqn:H_a_eq_src.
+          -- apply Z.eqb_eq in H_a_eq_src. rewrite <- H_a_eq_src. intros.
+            assert (Token.allowance s a (Caller ENV') = 0). auto.
+            assert (Caller ENV' <> src) as H_caller_neq_src. { destructAnds. assumption. }
+            destruct H_conds. apply H_iff3 in H_caller_neq_src. 
+            assert (amount = 0). { apply Z.le_antisymm; try lia.
+              rewrite <- H_a_eq_src in H_caller_neq_src. rewrite H0 in H_caller_neq_src. lia.
+            }
+            destruct (i =? Caller ENV'); try lia; auto.
+          -- assumption.
+    - unfold Relation_Definitions.reflexive. auto.
+    - unfold Relation_Definitions.transitive. auto.
 Qed.
 
-Lemma swap0_post1_witness : swap0_post1.
+
+Definition Amm_allowance_zero_Prop (ENV : Env) (T0 T1 : Token.State) (L : Z) (NextAddr : address) (STATE : State) : Prop :=
+  forall i, i <> Amm.addr STATE
+  -> Token.allowance (Amm.token0 STATE) (Amm.addr STATE) i = 0 /\
+    Token.allowance (Amm.token1 STATE) (Amm.addr STATE) i = 0.
+
+Definition Amm_const_addr_Prop (ENV : Env) (T0 T1 : Token.State) (L : Z) (NextAddr : address) (STATE : State) : Prop :=
+  This ENV = Amm.addr STATE.
+
+Definition Amm_liq_incr_Prop  (ENV : Env) (T0 T1 : Token.State) (L : Z) (NextAddr : address) (STATE : State) : Prop :=
+  ((((Token.balanceOf T0) (This ENV)) * ((Token.balanceOf T1) (This ENV))) <= (((Token.balanceOf (Amm.token0 STATE)) (This ENV)) * ((Token.balanceOf (Amm.token1 STATE)) (This ENV)))).
+
+Definition Amm_balance_ge_reserve_0_Prop (ENV: Env) (T0 T1 : Token.State) (L : Z) (NextAddr : address) (STATE : State) : Prop :=
+  reserve0 STATE <= Token.balanceOf (token0 STATE) (addr STATE).
+
+Definition Amm_balance_ge_reserve_1_Prop (ENV: Env) (T0 T1 : Token.State) (L : Z) (NextAddr : address) (STATE : State) : Prop :=
+  reserve1 STATE <= Token.balanceOf (token1 STATE) (addr STATE).
+
+Definition IP (ENV : Env) (T0 T1 : Token.State) (L : Z) (NextAddr : address) (STATE : State) : Prop :=
+  Amm_allowance_zero_Prop ENV T0 T1 L NextAddr STATE
+  /\ Amm_const_addr_Prop ENV T0 T1 L NextAddr STATE
+  /\ Amm_liq_incr_Prop ENV T0 T1 L NextAddr STATE.
+
+Lemma Amm_allowance_zero_init : invariantInit Amm_allowance_zero_Prop.
 Proof.
-  intros NA NA' ENV STATE STATE' amt HConds Hreach Htransition.
-  destruct HConds.
-  destruct Htransition; simpl.
-  - destructAnds. convert_neq. rewrite_eqs.
-    rewrite Z.eqb_refl.
-    apply mod_prop. lia.
-  - destructAnds. convert_neq. rewrite_eqs.
-    rewrite Z.eqb_refl.
-    apply mod_prop; lia.
+  intros ENV T0 T1 L NextAddr A NextAddr' Hconstr i Hi_neq.
+  simpl in *.
+  split.
+  - apply ERC20_allowance_zero with (Before := addr A).
+    + assumption.
+    + destruct Hconstr; destruct H_conds. assumption.
+    + reflexivity.
+  - apply ERC20_allowance_zero with (Before := addr A).
+    + assumption.
+    + destruct Hconstr; destruct H_conds. assumption.
+    + reflexivity.
+Qed.
+
+
+Ltac rewrite_eqb H :=
+  match H with
+  | _ =? _ = true => apply Z.eqb_eq in H as H'; rewrite H'
+  | _ =? _ = false => apply Z.eqb_neq in H as H'; rewrite H'
+  end.
+
+Lemma Amm_allowance_zero_step : invariantStep Amm_allowance_zero_Prop.
+Proof.
+  unfold invariantStep, Amm_allowance_zero_Prop.
+  intros ENV0 T0 T1 L NextAddr0 STATE0 STATE0' HinitPrecs Hstep Hyp i Hi_neq.
+  destruct Hstep as [ENV0' [NextAddr [NextAddr' Htransition]]].
+  destruct Htransition
+    as [ 
+       | _ _ Hcaller_cnstr _ HTokenTransition Haddr_const _ _ _ _ _ Htk1_const
+       | _ _ Hcaller_cnstr _ HTokenTransition Haddr_const _ _ _ _ _ Htk0_const].
+  - destruct H; destruct H; simpl; auto.
+  - destruct HTokenTransition; destruct H0; rewrite <- Haddr_const in *; rewrite <- Htk1_const.
+    + destruct H0; simpl; auto.
+    + (* transferFrom *)
+      destruct H0; simpl; auto.
+      * destruct (addr STATE0 =? src) eqn:Hif_cond1, (i =? Caller ENV0')%bool eqn:Hif_cond2; auto.
+        -- (* true, true *)
+        assert (Caller ENV0' <> src) as H_caller_neq_src; [lia|].
+        assert (addr STATE0 = src) as HstateCallerEq; [lia|].
+        assert (i = Caller ENV0') as HiCallerEq; [lia|].
+        destruct H_conds.
+        rewrite <- HstateCallerEq in *.
+        rewrite <- HiCallerEq in *.
+        apply Hyp in Hi_neq as Hyp'.
+        apply H_iff3 in H_caller_neq_src as Hamt_prec.
+        assert (amount = 0). lia.
+        simpl.
+        split; lia.
+        -- (* true, false*)
+        apply Z.eqb_eq in Hif_cond1 as Hif_cond1'; rewrite <- Hif_cond1'; auto.
+      * destruct (addr STATE0 =? src) eqn:Hif_cond1, (i =? Caller ENV0')%bool eqn:Hif_cond2; auto.
+        -- (* true, true *)
+        assert (Caller ENV0' <> src) as H_caller_neq_src; [lia|].
+        assert (addr STATE0 = src) as HstateCallerEq; [lia|].
+        assert (i = Caller ENV0') as HiCallerEq; [lia|].
+        destruct H_conds.
+        rewrite <- HstateCallerEq in *.
+        rewrite <- HiCallerEq in *.
+        apply Hyp in Hi_neq as Hyp'.
+        apply H_iff3 in H_caller_neq_src as Hamt_prec.
+        assert (amount = 0). lia.
+        simpl.
+        split; lia.
+        -- (* true, false*)
+        apply Z.eqb_eq in Hif_cond1 as Hif_cond1'; rewrite <- Hif_cond1'; auto.
+    + (* approve *)
+      destruct H0; simpl.
+      * assert (Caller ENV0' =? addr STATE0 = false). {
+          rewrite Z.eqb_neq.
+          destruct H_conds.
+          apply Hcaller_cnstr.
+          constructor. }
+        rewrite Z.eqb_sym in H0; rewrite H0.
+        apply Hyp; auto.
+      * apply Hyp; auto.
+    + destruct H0; simpl; auto.
+    + destruct H0; simpl; auto.
+      * destruct (addr STATE0 =? src) eqn:Hif_cond1, (i =? Caller ENV0')%bool eqn:Hif_cond2; auto.
+        -- (* true, true *)
+        assert (Caller ENV0' <> src) as H_caller_neq_src; [lia|].
+        assert (addr STATE0 = src) as HstateCallerEq; [lia|].
+        assert (i = Caller ENV0') as HiCallerEq; [lia|].
+        destruct H_conds.
+        rewrite <- HstateCallerEq in *.
+        rewrite <- HiCallerEq in *.
+        apply Hyp in Hi_neq as Hyp'.
+        apply H_iff3 in H_caller_neq_src as Hamt_prec.
+        assert (amount = 0). lia.
+        simpl.
+        split; lia.
+        -- (* true, false*)
+        apply Z.eqb_eq in Hif_cond1 as Hif_cond1'; rewrite <- Hif_cond1'; auto.
+    + (* mint *)
+      destruct H0; simpl; auto.
+    + destruct H0; simpl; auto.
+    + destruct H0; simpl; auto.
+    + destruct H0; simpl; auto.
+  - destruct HTokenTransition; destruct H0; rewrite <- Haddr_const in *; rewrite <- Htk0_const.
+    + destruct H0; simpl; auto.
+    + (* transferFrom *)
+      destruct H0; simpl; auto.
+      * destruct (addr STATE0 =? src) eqn:Hif_cond1, (i =? Caller ENV0')%bool eqn:Hif_cond2; auto.
+        -- (* true, true *)
+        assert (Caller ENV0' <> src) as H_caller_neq_src; [lia|].
+        assert (addr STATE0 = src) as HstateCallerEq; [lia|].
+        assert (i = Caller ENV0') as HiCallerEq; [lia|].
+        destruct H_conds.
+        rewrite <- HstateCallerEq in *.
+        rewrite <- HiCallerEq in *.
+        apply Hyp in Hi_neq as Hyp'.
+        apply H_iff3 in H_caller_neq_src as Hamt_prec.
+        assert (amount = 0). lia.
+        simpl.
+        split; lia.
+        -- (* true, false*)
+        apply Z.eqb_eq in Hif_cond1 as Hif_cond1'; rewrite <- Hif_cond1'; auto.
+      * destruct (addr STATE0 =? src) eqn:Hif_cond1, (i =? Caller ENV0')%bool eqn:Hif_cond2; auto.
+        -- (* true, true *)
+        assert (Caller ENV0' <> src) as H_caller_neq_src; [lia|].
+        assert (addr STATE0 = src) as HstateCallerEq; [lia|].
+        assert (i = Caller ENV0') as HiCallerEq; [lia|].
+        destruct H_conds.
+        rewrite <- HstateCallerEq in *.
+        rewrite <- HiCallerEq in *.
+        apply Hyp in Hi_neq as Hyp'.
+        apply H_iff3 in H_caller_neq_src as Hamt_prec.
+        assert (amount = 0). lia.
+        simpl.
+        split; lia.
+        -- (* true, false*)
+        apply Z.eqb_eq in Hif_cond1 as Hif_cond1'; rewrite <- Hif_cond1'; auto.
+    + (* approve *)
+      destruct H0; simpl.
+      * assert (Caller ENV0' =? addr STATE0 = false). {
+          rewrite Z.eqb_neq.
+          destruct H_conds.
+          apply Hcaller_cnstr.
+          constructor. }
+        rewrite Z.eqb_sym in H0; rewrite H0.
+        apply Hyp; auto.
+      * apply Hyp; auto.
+    + destruct H0; simpl; auto.
+    + destruct H0; simpl; auto.
+      * destruct (addr STATE0 =? src) eqn:Hif_cond1, (i =? Caller ENV0')%bool eqn:Hif_cond2; auto.
+        -- (* true, true *)
+        assert (Caller ENV0' <> src) as H_caller_neq_src; [lia|].
+        assert (addr STATE0 = src) as HstateCallerEq; [lia|].
+        assert (i = Caller ENV0') as HiCallerEq; [lia|].
+        destruct H_conds.
+        rewrite <- HstateCallerEq in *.
+        rewrite <- HiCallerEq in *.
+        apply Hyp in Hi_neq as Hyp'.
+        apply H_iff3 in H_caller_neq_src as Hamt_prec.
+        assert (amount = 0). lia.
+        simpl.
+        split; lia.
+        -- (* true, false*)
+        apply Z.eqb_eq in Hif_cond1 as Hif_cond1'; rewrite <- Hif_cond1'; auto.
+    + destruct H0; simpl; auto.
+    + destruct H0; simpl; auto.
+    + destruct H0; simpl; auto.
+    + destruct H0; simpl; auto.
+Qed.
+
+Lemma Amm_addr_constant_init : invariantInit Amm_const_addr_Prop.
+Proof.
+  intros ENV t0 t1 L NextAddr STATE STATE' Hconstr.
+  destruct Hconstr.
+  unfold Amm_const_addr_Prop.
+  simpl.
+  destruct H_conds.
+  auto.
+Qed.
+
+Lemma Amm_addr_constant_step : invariantStep Amm_const_addr_Prop.
+Proof.
+  intros ENV0 T0 T1 L NextAddr0 STATE STATE' HinitPrecs Hstep Hyp.
+  unfold Amm_const_addr_Prop.
+  destruct Hstep as [ENV [NextAddr [NextAddr' Htransition]]].
+  destruct Htransition
+    as [ HAmmStep
+       | Hnac Horgc Hcallerc _ HTokenExtStep Haddr_const _ _ _ _ _ Htk1_const
+       | Hnac Horgc Hcallerc _ HTokenExtStep Haddr_const _ _ _ _ _ Htk0_const ].
+  - destruct HAmmStep; destruct H; auto.
+  - destruct HTokenExtStep; rewrite <- Haddr_const; simpl; auto.
+  - destruct HTokenExtStep; rewrite <- Haddr_const; simpl; auto.
+Qed.
+
+Definition Amm_balance_ge_reserve_0_AssistedProp (ENV: Env) (T0 T1 : Token.State) (L : Z) (NextAddr : address) (STATE : State) : Prop :=
+  Amm_const_addr_Prop ENV T0 T1 L NextAddr STATE /\
+  Amm_allowance_zero_Prop ENV T0 T1 L NextAddr STATE /\
+  Amm_balance_ge_reserve_0_Prop ENV T0 T1 L NextAddr STATE.
+
+Lemma Amm_balance_ge_reserve_0_init : invariantInit Amm_balance_ge_reserve_0_AssistedProp.
+Proof.
+  intros ENV t0 t1 L NextAddr STATE NextAddr' Hconstr.
+  unfold Amm_balance_ge_reserve_0_AssistedProp, Amm_balance_ge_reserve_0_Prop.
+  split. assert (invariantInit Amm_const_addr_Prop); eapply Amm_addr_constant_init. eassumption.
+  split. assert (invariantInit Amm_allowance_zero_Prop); eapply Amm_allowance_zero_init; eassumption.
+  destruct Hconstr, H_conds; simpl. auto.
+  rewrite H_This_eq_NextAddr.
+  reflexivity.
+Qed.
+
+Lemma Amm_balance_ge_reserve_0_step : invariantStep Amm_balance_ge_reserve_0_AssistedProp.
+Proof.
+  intros ENV0 t0 t1 L NextAddr0 STATE STATE' H_conds0 Hstep [Hyp1 [Hyp2 Hyp3]].
+  unfold Amm_balance_ge_reserve_0_AssistedProp, Amm_balance_ge_reserve_0_Prop.
+  split. assert (invariantStep Amm_const_addr_Prop); eapply Amm_addr_constant_step; eassumption.
+  split. assert (invariantStep Amm_allowance_zero_Prop); eapply Amm_allowance_zero_step; eassumption.
+  simpl.
+  destruct Hstep as [ENV [NextAddr [NextAddr' Htransition]]].
+  destruct Htransition
+    as [ HAmmStep
+       | Hnac Horgc Hcallerc _ HTokenTransition Haddr_const _ _ _ Hres0_const _ Htk1_const
+       | Hnac Horgc Hcallerc _ HTokenTransition Haddr_const _ _ _ Hres0_const _ Htk0_const ].
+  - destruct HAmmStep; auto; try now (destruct H; simpl; auto).
+    + (* swap0 *)
+      destruct H; destruct H_conds; simpl; rewrite <- H_This_eq_addState; reflexivity.
+    + (* swap1 *)
+      destruct H; destruct H_conds; simpl; [ rewrite_eqbs | rewrite H_This_eq_addState ]; reflexivity.
+    + (* mint *)
+      destruct H; destruct H_conds; rewrite H_This_eq_addState; simpl; reflexivity.
+    + (* burn *)
+      destruct H; destruct H_conds; simpl; [ rewrite_eqbs | rewrite H_This_eq_addState ]; reflexivity.  
+  - assert (addr STATE <> Caller ENV) as H_addrState_neq_caller;
+      [apply Z.neq_sym; apply Hcallerc; constructor|].
+    rewrite <- Haddr_const, <- Hres0_const.
+    destruct HTokenTransition as [HTokenTransition]; destruct HTokenTransition; try now (destruct H0; simpl; auto).
+    + (* transfer *)
+      destruct H0; simpl; auto.
+      * rewrite_eqbs.
+        destruct (addr STATE =? to) eqn:Hifcond0; simpl; auto.
+        -- eapply Z.le_trans. apply Hyp3. apply Z.eqb_eq in Hifcond0; rewrite Hifcond0. destruct H_conds; lia. 
+    +  (* transferFrom *)
+      destruct H0; simpl; auto.
+      * destruct (addr STATE =? src) eqn:Hifcond0, (addr STATE =? dst) eqn:Hifcond1.
+        -- assert (amount = 0); lia.
+        -- assert (amount = 0); lia.
+        -- eapply Z.le_trans. apply Hyp3. rewrite_b_right Hifcond1. destruct H_conds; lia. 
+        -- apply Hyp3.
+      * destruct (addr STATE =? src) eqn:Hifcond0, (addr STATE =? dst) eqn:Hifcond1.
+        -- assert (amount = 0); lia.
+        -- destruct H_conds. 
+          rewrite_b_right Hif_cond0.
+          assert (amount = 0). {
+            assert (Token.allowance (token0 STATE) (addr STATE) (Caller ENV) = 0); [apply Hyp2; auto|].
+            rewrite H0 in H_iff3. lia.
+          }   
+          rewrite H0. unfold Amm_balance_ge_reserve_0_Prop in *. rewrite Hyp3; lia.
+        -- eapply Z.le_trans. apply Hyp3. rewrite_b_right Hifcond1. destruct H_conds; lia. 
+        -- apply Hyp3.
+      * destruct (addr STATE =? src) eqn:Hifcond0, (addr STATE =? dst) eqn:Hifcond1.
+        -- assert (amount = 0); lia.
+        -- destruct H_conds. 
+          rewrite_b_right Hif_cond0.
+          assert (amount = 0). {
+            assert (Token.allowance (token0 STATE) (addr STATE) (Caller ENV) = 0); [apply Hyp2; auto|].
+            rewrite H0 in H_iff3. lia.
+          }   
+          rewrite H0. unfold Amm_balance_ge_reserve_0_Prop in *. rewrite Hyp3; lia.
+        -- eapply Z.le_trans. apply Hyp3. apply Z.eqb_eq in Hifcond1; rewrite Hifcond1. destruct H_conds; lia. 
+        -- apply Hyp3.
+    +  (* burn *)
+      destruct H0; simpl; auto.
+      * rewrite_eqbs. auto.
+    +  (* burnFrom *)
+      destruct H0; simpl; auto.
+      * destruct (addr STATE =? src) eqn:Hifcond.
+        -- assert (amount = 0). { destruct H_conds.
+            bool_to_prop. rewrite <- Hifcond in H_iff3. unfold Amm_allowance_zero_Prop in Hyp2. specialize Hyp2 with (i := Caller ENV) as Hyp2'. lia. }
+            rewrite H0. rewrite_b_right Hifcond. unfold Amm_balance_ge_reserve_0_Prop in Hyp3. lia.
+        -- destruct H; simpl; auto.
+      * destruct (addr STATE =? src) eqn:Hifcond.
+        -- assert (amount = 0). { destruct H_conds.
+            bool_to_prop. rewrite <- Hifcond in H_iff3. unfold Amm_allowance_zero_Prop in Hyp2. specialize Hyp2 with (i := Caller ENV) as Hyp2'. lia. }
+            rewrite H0. rewrite_b_right Hifcond. unfold Amm_balance_ge_reserve_0_Prop in Hyp3. lia.
+        -- destruct H; simpl; auto.
+      * destruct (addr STATE =? src) eqn:Hifcond.
+        -- assert (amount = 0); lia.
+        -- destruct H; simpl; auto.
+    +  (* mint *)
+      destruct H0; simpl; auto.
+      * rewrite_eqbs.
+        destruct (addr STATE =? dst) eqn:Hifcond0; simpl; auto.
+        -- eapply Z.le_trans. apply Hyp3. apply Z.eqb_eq in Hifcond0; rewrite Hifcond0. destruct H_conds; lia. 
+  - destruct HTokenTransition; 
+    simpl; rewrite <- Haddr_const, <- Hres0_const, <- Htk0_const; assumption.
+Qed.
+
+
+Definition Amm_balance_ge_reserve_1_AssistedProp (ENV: Env) (T0 T1 : Token.State) (L : Z) (NextAddr : address) (STATE : State) : Prop :=
+  Amm_const_addr_Prop ENV T0 T1 L NextAddr STATE /\
+  Amm_allowance_zero_Prop ENV T0 T1 L NextAddr STATE /\
+  Amm_balance_ge_reserve_1_Prop ENV T0 T1 L NextAddr STATE.
+
+Lemma Amm_balance_ge_reserve_1_init : invariantInit Amm_balance_ge_reserve_1_AssistedProp.
+Proof.
+  intros ENV t0 t1 L NextAddr0 STATE NextAddr0' Hconstr.
+  unfold Amm_balance_ge_reserve_1_AssistedProp, Amm_balance_ge_reserve_1_Prop.
+  split. assert (invariantInit Amm_const_addr_Prop); eapply Amm_addr_constant_init; eassumption.
+  split. assert (invariantInit Amm_allowance_zero_Prop); eapply Amm_allowance_zero_init; eassumption.
+  destruct Hconstr, H_conds; simpl. auto.
+  rewrite H_This_eq_NextAddr.
+  reflexivity.
+Qed.
+
+Lemma Amm_balance_ge_reserve_1_step : invariantStep Amm_balance_ge_reserve_1_AssistedProp.
+Proof.
+  intros ENV0 t0 t1 L NextAddr0 STATE STATE' H_conds0 Hstep [Hyp1 [Hyp2 Hyp3]].
+  unfold Amm_balance_ge_reserve_1_AssistedProp, Amm_balance_ge_reserve_1_Prop.
+  split. assert (invariantStep Amm_const_addr_Prop); eapply Amm_addr_constant_step; eassumption.
+  split. assert (invariantStep Amm_allowance_zero_Prop); eapply Amm_allowance_zero_step; eassumption.
+  simpl.
+  destruct Hstep as [ENV [NextAddr [NextAddr' Htransition]]].
+  destruct Htransition
+    as [ HAmmStep
+       | Hnac Horgc Hcallerc _ HTokenTransition Haddr_const _ _ _ _ Hres1_const Htk1_const
+       | Hnac Horgc Hcallerc _ HTokenTransition Haddr_const _ _ _ _ Hres1_const Htk0_const ].
+  - destruct HAmmStep; auto; try now (destruct H; simpl; auto).
+    + (* swap0 *)
+      destruct H; destruct H_conds; simpl; [ rewrite_eqbs | rewrite H_This_eq_addState ]; reflexivity.
+    + (* swap1 *)
+      destruct H; destruct H_conds; simpl; rewrite <- H_This_eq_addState; reflexivity.
+    + (* mint *)
+      destruct H; destruct H_conds; rewrite H_This_eq_addState; simpl; reflexivity.
+    + (* burn *)
+      destruct H; destruct H_conds; simpl; [ rewrite_eqbs | rewrite H_This_eq_addState ]; reflexivity.  
+  - destruct HTokenTransition; 
+    simpl; rewrite <- Haddr_const, <- Hres1_const, <- Htk1_const; assumption.
+  - assert (addr STATE <> Caller ENV) as H_addrState_neq_caller;
+      [apply Z.neq_sym; apply Hcallerc; constructor|].
+    rewrite <- Haddr_const, <- Hres1_const.
+    destruct HTokenTransition as [HTokenTransition]; destruct HTokenTransition; try now (destruct H0; simpl; auto).
+    + (* transfer *)
+      destruct H0; simpl; auto.
+      * rewrite_eqbs.
+        destruct (addr STATE =? to) eqn:Hifcond0; simpl; auto.
+        -- eapply Z.le_trans. apply Hyp3. apply Z.eqb_eq in Hifcond0; rewrite Hifcond0. destruct H_conds; lia. 
+    +  (* transferFrom *)
+      destruct H0; simpl; auto.
+      * destruct (addr STATE =? src) eqn:Hifcond0, (addr STATE =? dst) eqn:Hifcond1.
+        -- assert (amount = 0); lia.
+        -- assert (amount = 0); lia.
+        -- eapply Z.le_trans. apply Hyp3. rewrite_b_right Hifcond1. destruct H_conds; lia. 
+        -- apply Hyp3.
+      * destruct (addr STATE =? src) eqn:Hifcond0, (addr STATE =? dst) eqn:Hifcond1.
+        -- assert (amount = 0); lia.
+        -- destruct H_conds. 
+          rewrite_b_right Hif_cond0.
+          assert (amount = 0). {
+            assert (Token.allowance (token1 STATE) (addr STATE) (Caller ENV) = 0); [apply Hyp2; auto|].
+            rewrite H0 in H_iff3. lia.
+          }   
+          rewrite H0. unfold Amm_balance_ge_reserve_1_Prop in *. rewrite Hyp3; lia.
+        -- eapply Z.le_trans. apply Hyp3. rewrite_b_right Hifcond1. destruct H_conds; lia. 
+        -- apply Hyp3.
+      * destruct (addr STATE =? src) eqn:Hifcond0, (addr STATE =? dst) eqn:Hifcond1.
+        -- assert (amount = 0); lia.
+        -- destruct H_conds. 
+          rewrite_b_right Hif_cond0.
+          assert (amount = 0). {
+            assert (Token.allowance (token1 STATE) (addr STATE) (Caller ENV) = 0); [apply Hyp2; auto|].
+            rewrite H0 in H_iff3. lia.
+          }   
+          rewrite H0. unfold Amm_balance_ge_reserve_1_Prop in *. rewrite Hyp3; lia.
+        -- eapply Z.le_trans. apply Hyp3. apply Z.eqb_eq in Hifcond1; rewrite Hifcond1. destruct H_conds; lia. 
+        -- apply Hyp3.
+    + (* burn *)
+      destruct H0; simpl; auto.
+      * rewrite_eqbs. apply Hyp3.
+    + (* burnFrom *)
+      destruct H0; simpl; auto.
+      * destruct (addr STATE =? src) eqn:Hifcond.
+        -- assert (amount = 0). { destruct H_conds.
+            bool_to_prop. rewrite <- Hifcond in H_iff3. unfold Amm_allowance_zero_Prop in Hyp2. specialize Hyp2 with (i := Caller ENV) as Hyp2'. lia. }
+            rewrite H0. rewrite_b_right Hifcond. unfold Amm_balance_ge_reserve_1_Prop in Hyp3. lia.
+        -- apply Hyp3.
+      * destruct (addr STATE =? src) eqn:Hifcond.
+        -- assert (amount = 0). { destruct H_conds.
+            bool_to_prop. rewrite <- Hifcond in H_iff3. unfold Amm_allowance_zero_Prop in Hyp2. specialize Hyp2 with (i := Caller ENV) as Hyp2'. lia. }
+            rewrite H0. rewrite_b_right Hifcond. unfold Amm_balance_ge_reserve_1_Prop in Hyp3. lia.
+        -- apply Hyp3.
+      * destruct (addr STATE =? src) eqn:Hifcond.
+        -- assert (amount = 0); lia.
+        -- apply Hyp3.
+    + (* mint *)
+      destruct H0; simpl; auto.
+      * destruct (addr STATE =? dst) eqn:Hifcond.
+        -- eapply Z.le_trans. apply Hyp3. rewrite_b_right Hifcond1. destruct H_conds; lia. 
+        -- apply Hyp3.
+Qed.
+
+
+
+
+Fixpoint balanceOf_sum' (balanceOf : address -> Z) (n : nat) (acc : Z) : Z :=
+    match n with
+    | O => balanceOf 0 + acc
+    | S n => balanceOf_sum' balanceOf n (acc + balanceOf (Z.of_nat (S n)))
+    end.
+
+Definition balanceOf_sum (STATE : State) :=
+  balanceOf_sum' (balanceOf STATE) (Z.to_nat MAX_ADDRESS) 0.
+
+
+Definition transfer_from map (from : address) (amt : Z) :=
+  fun b => if b =? from then map from - amt else map b.
+
+Definition transfer_to map (from : address) (amt : Z) :=
+  fun b => if b =? from then map from + amt else map b.
+
+Definition transfer map from to amt := transfer_to (transfer_from map from amt) to amt.
+
+Definition transfer' map from to amt := transfer_from (transfer_to map to amt) from amt.
+
+Lemma balanceOf_sum_f_eq f f' addr acc :
+  (forall x, x <= Z.of_nat addr -> f x = f' x) ->
+  balanceOf_sum' f addr acc = balanceOf_sum' f' addr acc.
+Proof.
+  revert acc. induction addr; intros acc Hyp.
+  - simpl. rewrite Hyp. reflexivity. lia.
+  - simpl. rewrite IHaddr. rewrite Hyp. reflexivity.
+    lia. intros. eapply Hyp. lia.
+Qed.
+
+Lemma balanceOf_sum_acc f  addr acc z :
+  balanceOf_sum' f addr (acc + z) = balanceOf_sum' f addr acc + z.
+Proof.
+  revert z acc. induction addr; intros z acc.
+  - simpl. lia.
+  - simpl. rewrite !IHaddr. lia.
+Qed.
+
+Opaque Z.sub Z.add Z.of_nat.
+
+Lemma balanceOf_sum_thm x f f' addr acc :
+  (forall y, x <> y -> f y = f' y) ->
+  0 <= x ->
+  balanceOf_sum' f addr acc =
+  if (Z.to_nat x <=? addr)%nat then balanceOf_sum' f' addr acc - f' x + f x else balanceOf_sum' f' addr acc.
+Proof.
+  revert acc. induction addr; intros acc Hyp Hleq1.
+  - simpl. destruct (0 =? x) eqn:Heq.
+    + eapply Z.eqb_eq in Heq. subst.
+      simpl. lia.
+    + eapply Z.eqb_neq in Heq.
+      assert (Hbeq : (Z.to_nat x <=? 0)%nat = false).
+      { eapply leb_correct_conv. lia. }
+      rewrite Hbeq. rewrite Hyp. reflexivity. eauto.
+
+  - destruct (Z.to_nat x <=? S addr0)%nat eqn:Hleq.
+    + eapply Nat.leb_le in Hleq.
+      destruct (Z.of_nat (S addr0) =? x) eqn:Heqb.
+      * eapply Z.eqb_eq in Heqb. simpl. rewrite Heqb.
+        erewrite balanceOf_sum_f_eq with (f' := f').
+        rewrite !balanceOf_sum_acc. lia.
+
+        intros. eapply Hyp. lia.
+
+      * simpl.
+        destruct ((Z.to_nat x <=? addr0)%nat) eqn:Hleq'.
+        -- rewrite IHaddr; eauto. rewrite Hyp. reflexivity.
+           intros Heq; subst. lia.
+        -- eapply Z.eqb_neq in Heqb.
+           eapply Nat.leb_gt in Hleq'. lia.
+
+    + simpl. eapply leb_complete_conv in Hleq.
+      erewrite balanceOf_sum_f_eq with (f' := f').
+      rewrite Hyp. reflexivity.
+      * intros Heq; subst. lia.
+      * intros. rewrite Hyp. reflexivity.
+        intros Heq; subst. lia.
+Qed.
+
+Lemma balanceOf_sum_thm' x f f' acc :
+  (forall y, x <> y -> f y = f' y) ->
+  0 <= x <= MAX_ADDRESS->
+  balanceOf_sum' f (Z.to_nat MAX_ADDRESS) acc = balanceOf_sum' f' (Z.to_nat MAX_ADDRESS) acc - f' x + f x.
+Proof.
+  intros H_f [H_x_0 H_x_max].
+  rewrite balanceOf_sum_thm with (x := x) (f' := f').
+  - apply Z2Nat.inj_le in H_x_max; try lia.
+    rewrite <- Nat.leb_le in H_x_max.
+    rewrite H_x_max.
+    reflexivity.
+  - assumption.
+  - assumption.
+Qed.
+
+Lemma balanceOf_sum_transfer_thm x1 x2 f f' acc :
+  (forall y, x1 <> y -> x2 <> y -> f y = f' y) ->
+  f x1 + f x2 = f' x1 + f' x2 ->
+  0 <= x1 <= MAX_ADDRESS ->
+  0 <= x2 <= MAX_ADDRESS ->
+  balanceOf_sum' f (Z.to_nat MAX_ADDRESS) acc = balanceOf_sum' f' (Z.to_nat MAX_ADDRESS) acc.
+Proof.
+  intros H_f1 H_f2 [H_x1_0 H_x1_max] [H_x2_0 H_x2_max].
+  rewrite balanceOf_sum_thm with (x := x1) (f' := fun _b => if _b =? x1 then f' _b else f _b).
+  - apply Z2Nat.inj_le in H_x1_max; try lia.
+    rewrite <- Nat.leb_le in H_x1_max.
+    rewrite H_x1_max, Z.eqb_refl.
+    rewrite balanceOf_sum_thm with (x := x2) (f' := f').
+    + apply Z2Nat.inj_le in H_x2_max; try lia.
+      rewrite <- Nat.leb_le in H_x2_max.
+      rewrite H_x2_max.
+      destruct (x2 =? x1) eqn:Hx2x1.
+      * apply Z.eqb_eq in Hx2x1. subst. lia.
+      * lia.
+    + intros. destruct (y =? x1) eqn:Hyx1.
+      * lia.
+      * apply H_f1; [lia | assumption].
+    + lia.
+  - intros. destruct (y =? x1) eqn:Hyx1.
+    * apply H_f1; [assumption | lia].
+    * reflexivity.
   - lia.
 Qed.
 
-Lemma swap1_post0_witness : swap1_post0.
+
+Theorem initialSupply': forall ENV _totalSupply t0 t1 NextAddr State NextAddr' (n : nat),
+    0 <= Caller ENV ->
+    0 <= This ENV ->
+    Caller ENV < This ENV ->
+    constructor ENV t0 t1 _totalSupply NextAddr State NextAddr' ->
+    balanceOf_sum' (balanceOf (State)) n 0 =
+    if (Z.of_nat n <? (Caller ENV)) then 0 else
+    if (Z.of_nat n <? (This ENV)) then totalSupply State - 1000 else
+    totalSupply State.
 Proof.
-  intros NA NA' ENV STATE STATE' amt HConds Hreach Htransition.
-  destruct HConds.
-  destruct Htransition; simpl.
-  - destructAnds. convert_neq. rewrite_eqs.
-    rewrite Z.eqb_refl.
-    apply mod_prop2; lia.
-  - destructAnds. convert_neq. rewrite_eqs.
-    rewrite Z.eqb_refl.
-    apply mod_prop2; lia.
-  - reflexivity.
+  intros ENV ? ? ? ? ? ? ? _ _ _ Hcnstr.
+  destruct Hcnstr as [? H_conds _ _]; simpl.
+
+  assert (forall n : nat, Z.of_nat n < Caller ENV ->
+      balanceOf_sum' (fun _binding_0 : address => if _binding_0 =? This ENV then 1000 else if _binding_0 =? Caller ENV then _totalSupply - 1000 else 0) n 0 = 0) as H0.
+  { intros. induction n0.
+    - simpl. destruct H_conds. destruct (Caller ENV), (This ENV); lia; discriminate.
+    - simpl. rewrite -> balanceOf_sum_acc. destruct H_conds.
+      destruct (Z.of_nat (S n0) =? Caller ENV) eqn:Heq.
+      + apply Z.eqb_eq in Heq. apply Z.lt_neq in H. contradiction.
+      + rewrite IHn0.
+        * destruct (Z.of_nat (S n0) =? This ENV) eqn:Heq'; try lia.
+          -- apply Z.eqb_eq in Heq'. lia.
+        * lia.
+  }
+
+  induction n.
+  - destruct H_conds; simpl.
+    assert (forall p, Z.of_nat 0 <? Z.pos p = true) as Hmy; [auto|].
+    destruct (Caller ENV) eqn:Hcaller, (This ENV) eqn:Hthis; try lia.
+    + rewrite Z.ltb_irrefl; rewrite Hmy; lia.
+    + rewrite Hmy; lia.
+  - simpl. rewrite balanceOf_sum_acc.
+    destruct (Z.of_nat (S n) <? Caller ENV) eqn:Hlt.
+    + destruct (Z.of_nat (S n) =? Caller ENV) eqn:Heq. * lia.
+      * rewrite H0.
+        -- destruct (Z.of_nat (S n) =? This ENV) eqn:Heq'; try lia.
+          ++ destruct H_conds. apply Z.eqb_eq in Heq'. apply Z.ltb_lt in Hlt. lia.
+        -- apply Z.ltb_lt in Hlt. lia.
+    + destruct (Z.of_nat (S n) =? Caller ENV) eqn:Heq.
+      * rewrite H0.
+        -- destruct (Z.of_nat (S n) =? This ENV) eqn:Heq'; try lia.
+          ++ destruct H_conds. rewrite_b_left Heq'. lia.
+          ++ destruct (Z.of_nat (S n) <? This ENV) eqn:Hlt'; try lia. 
+            apply Z.ltb_ge in Hlt'.
+            apply Z.eqb_eq in Heq. rewrite Heq in *. destruct H_conds. lia.
+        -- apply Z.eqb_eq in Heq. rewrite <- Heq. lia.
+      * rewrite IHn.
+        assert ( Z.of_nat n <? Caller ENV = false).
+        { apply Z.ltb_ge in Hlt. apply Z.eqb_neq in Heq. lia. }
+        rewrite H.
+        destruct (Z.of_nat n <? This ENV) eqn:Hlt', (Z.of_nat (S n) =? This ENV) eqn:Heq'.
+        -- assert (Z.of_nat (S n) <? This ENV = false). lia.
+        rewrite H1. lia.
+        -- assert (Z.of_nat (S n) < This ENV) as Hlt''. bool_to_prop. lia.
+          prop_to_bool. rewrite Hlt''. lia.
+        -- bool_to_prop. lia.
+        -- assert (Z.of_nat (S n) <? This ENV = false); [apply Z.ltb_ge; lia|].
+           rewrite H1. lia.
 Qed.
 
-Lemma swap1_post1_witness : swap1_post1.
+Theorem initialSupply: forall ENV t0 t1 _totalSupply NextAddr STATE NextAddr',
+    0 <= Caller ENV <= MAX_ADDRESS ->
+    constructor ENV t0 t1 _totalSupply NextAddr STATE NextAddr' ->
+    balanceOf_sum STATE =
+    totalSupply STATE.
 Proof.
-  intros NA NA' ENV STATE STATE' amt HConds Hreach Htransition.
-  destruct HConds.
-  destruct Htransition; simpl.
-  - destructAnds. convert_neq. rewrite_eqs.
-    rewrite Z.eqb_refl.
-    apply div_prop2; lia.
-  - destructAnds. convert_neq. rewrite_eqs.
-    rewrite Z.eqb_refl.
-    apply div_prop2; lia.
-  - lia.
+  intros.
+  unfold balanceOf_sum.
+  (*destruct H0 as [? H_conds _ _].*)
+  erewrite -> initialSupply'; try (now eassumption); destruct H0 as [? H_conds _ _].
+  - rewrite Z2Nat.id.
+    + destruct (MAX_ADDRESS <? Caller ENV) eqn:Hineq.
+      * apply Z.ltb_lt in Hineq. lia.
+      * destruct (MAX_ADDRESS <? This ENV) eqn:Hineq'.
+        -- apply Z.ltb_lt in Hineq'.
+           destruct H_conds; unfold MAX_ADDRESS in *; lia.
+        -- reflexivity.
+    + unfold MAX_ADDRESS. unfold UINT_MAX. lia.
+  - destruct H_conds; lia.
+  - destruct H_conds; lia.
+  - destruct H_conds; lia.
 Qed.
 
+Theorem deltas: forall x1 x2 y1 y2,
+  x1 = y1 -> x1 - x2 = y1 - y2 -> x2 = y2.
+Proof.
+  intros. lia.
+Qed.
+
+
+Definition Amm_liqs_sum_eq_total_Prop (ENV : Env) (T0 T1 : Token.State) (L : Z) (NextAddr : address) (STATE : State) : Prop :=
+  balanceOf_sum STATE = totalSupply STATE.
+
+Definition Amm_liqs_sum_eq_total_AssistedProp (ENV: Env) (T0 T1 : Token.State) (L : Z) (NextAddr : address) (STATE : State) : Prop :=
+  Amm_const_addr_Prop ENV T0 T1 L NextAddr STATE /\
+  Amm_allowance_zero_Prop ENV T0 T1 L NextAddr STATE /\
+  Amm_balance_ge_reserve_0_AssistedProp ENV T0 T1 L NextAddr STATE /\
+  Amm_balance_ge_reserve_1_AssistedProp ENV T0 T1 L NextAddr STATE /\
+  Amm_liqs_sum_eq_total_Prop ENV T0 T1 L NextAddr STATE.
+
+Lemma Amm_liqs_sum_eq_total_init : invariantInit Amm_liqs_sum_eq_total_AssistedProp.
+Proof.
+  intros ENV t0 t1 L NextAddr State NexrAddr' Hconstr.
+  unfold Amm_liqs_sum_eq_total_AssistedProp, Amm_liqs_sum_eq_total_Prop.
+  split. assert (invariantInit Amm_const_addr_Prop); eapply Amm_addr_constant_init; eassumption.
+  split. assert (invariantInit Amm_allowance_zero_Prop); eapply Amm_allowance_zero_init; eassumption.
+  split. assert (invariantInit Amm_balance_ge_reserve_0_AssistedProp); eapply Amm_balance_ge_reserve_0_init; eassumption.
+  split. assert (invariantInit Amm_balance_ge_reserve_1_AssistedProp); eapply Amm_balance_ge_reserve_1_init; eassumption.
+  eapply initialSupply; [| eassumption].
+  destruct Hconstr as [? H_conds ? ?], H_conds; assumption.
+Qed.
+
+Lemma Amm_liqs_sum_eq_total_step : invariantStep Amm_liqs_sum_eq_total_AssistedProp.
+Proof.
+  intros ENV0 T0 T1 L NextAddr0 STATE STATE' HinitPrecs Hstep [Hyp1 [Hyp2 [Hyp3 [Hyp4 Hyp5]]]].
+  unfold Amm_liqs_sum_eq_total_AssistedProp, Amm_liqs_sum_eq_total_Prop in *.
+  split. assert (invariantStep Amm_const_addr_Prop); eapply Amm_addr_constant_step; eassumption.
+  split. assert (invariantStep Amm_allowance_zero_Prop); eapply Amm_allowance_zero_step; eassumption.
+  split. assert (invariantStep Amm_balance_ge_reserve_0_AssistedProp); eapply Amm_balance_ge_reserve_0_step; eassumption.
+  split. assert (invariantStep Amm_balance_ge_reserve_1_AssistedProp); eapply Amm_balance_ge_reserve_1_step; eassumption.
+  destruct Hstep as [ENV [NextAddr [NexteAddr' Htransition]]].
+  destruct Htransition
+    as [ HAmmStep
+       | Hnac Horgc Hcallerc _ HTokenExtStep Haddr_const _ _ Hbalance_const _ _ Htk1_const
+       | Hnac Horgc Hcallerc _ HTokenExtStep Haddr_const _ _ Hbalance_const _ _ Htk0_const ].
+  - destruct HAmmStep; simpl.
+    + (* swap0 *)
+      destruct H; simpl; auto.
+    + (* swap1 *)
+      destruct H; simpl; auto.
+    + (* mint *)
+      apply deltas with (x1 := balanceOf_sum STATE) (y1 := totalSupply STATE); [assumption|].
+      unfold balanceOf_sum. simpl.
+      rewrite balanceOf_sum_thm' with (x := to) (f' := balanceOf STATE').
+      * destruct H; simpl; rewrite Z.eqb_refl; lia.
+      * destruct H; simpl; intros; rewrite_eqbs; reflexivity.
+      * destruct H; simpl; unfold MAX_ADDRESS; destruct H_conds; lia.
+    + (* burn *)
+      apply deltas with (x1 := balanceOf_sum STATE) (y1 := totalSupply STATE); [assumption|].
+      unfold balanceOf_sum. simpl.
+      rewrite balanceOf_sum_thm' with (x := Caller ENV) (f' := balanceOf STATE').
+      * destruct H; simpl; rewrite Z.eqb_refl; lia.
+      * destruct H; simpl; intros; rewrite_eqbs; reflexivity.
+      * destruct H; simpl; unfold MAX_ADDRESS; destruct H_conds; lia.
+    + (* transfer *)
+      apply deltas with (x1 := balanceOf_sum STATE) (y1 := totalSupply STATE); [assumption|].
+      unfold balanceOf_sum. simpl.
+      rewrite balanceOf_sum_transfer_thm with (x1 := Caller ENV) (x2 := to) (f' := balanceOf STATE').
+      * destruct H; simpl; lia.
+      * destruct H; simpl; intros; rewrite_eqbs; reflexivity.
+      * destruct H; simpl; rewrite_eqbs; repeat rewrite Z.eqb_refl; lia.
+      * destruct H; simpl; unfold MAX_ADDRESS; destruct H_conds; lia.
+      * destruct H; simpl; unfold MAX_ADDRESS; destruct H_conds; lia.
+    + (* transferFrom *)
+      apply deltas with (x1 := balanceOf_sum STATE) (y1 := totalSupply STATE); [assumption|].
+      unfold balanceOf_sum. simpl.
+      rewrite balanceOf_sum_transfer_thm with (x1 := src) (x2 := dst) (f' := balanceOf STATE').
+      * destruct H; simpl; lia.
+      * destruct H; simpl; intros; rewrite_eqbs; reflexivity.
+      * destruct H; simpl; destructAnds; rewrite_eqbs; repeat rewrite Z.eqb_refl; lia.
+      * destruct H; simpl; unfold MAX_ADDRESS; destruct H_conds; lia.
+      * destruct H; simpl; unfold MAX_ADDRESS; destruct H_conds; lia.
+    + (* approve *)
+      destruct H; simpl; auto.
+    + (* totalSupply *)
+      destruct H; simpl; auto.
+    + (* balanceOf *)
+      destruct H; simpl; auto.
+    + (* allowance *)
+      destruct H; simpl; auto.
+  - destruct HTokenExtStep. unfold balanceOf_sum. rewrite <- H, <- Hbalance_const. assumption.
+  - destruct HTokenExtStep. unfold balanceOf_sum. rewrite <- H, <- Hbalance_const. assumption.
+Qed.
+
+Lemma Amm_liqs_sum_eq_total_reach : 
+  forall (ENV : Env) (t0 : Token.State) (t1 : Token.State) (liquidity : Z) (NextAddr : address) (STATE : State),
+     reachableFromInit ENV t0 t1 liquidity NextAddr STATE
+  -> Amm_liqs_sum_eq_total_AssistedProp ENV t0 t1 liquidity NextAddr STATE
+.
+Proof.
+  intros.
+  apply invariantReachable.
+  exact Amm_liqs_sum_eq_total_init.
+  exact Amm_liqs_sum_eq_total_step.
+  assumption.
+Qed.
+
+Lemma sum_mono :
+  forall f N M acc,
+  (forall (x : nat), (x <= M)%nat -> 0 <= f (Z.of_nat x))
+  -> (N <= M)%nat
+  -> balanceOf_sum' f N acc <= balanceOf_sum' f M acc.
+Proof.
+  intros f N M acc Hfnneg Hnm.
+  induction M.
+  - destruct N.
+    + reflexivity.
+    + lia.
+  - destruct (N ?= S M)%nat eqn:HnSm.
+    + apply Nat.compare_eq in HnSm.
+      subst. reflexivity.
+    + simpl. rewrite balanceOf_sum_acc.
+      rewrite <- Z.add_0_r at 1.
+      apply Z.add_le_mono.
+      * apply IHM; apply Nat.compare_lt_iff in HnSm.
+        -- intros. apply Hfnneg. lia.
+        -- lia.
+      * apply Hfnneg. lia.
+    + apply Nat.compare_gt_iff in HnSm.
+      lia.
+Qed.
+
+Lemma sum_pos :
+forall f n N,
+   (forall m, (m <= Z.of_nat N)-> 0 <= f m)
+-> (n <= N)%nat
+-> 0 <= balanceOf_sum' f n 0.
+Proof.
+intros.
+induction n.
+- unfold balanceOf_sum'.
+  rewrite Z.add_0_r.
+  apply H with (m := 0). lia.
+- simpl. rewrite balanceOf_sum_acc.
+  apply Z.add_nonneg_nonneg.
+  + apply IHn. lia.
+  + apply H. lia.
+Qed.
+
+Lemma sum_le_total' :
+forall f total n N,
+balanceOf_sum' f N 0 = total
+-> (n <= N)%nat
+-> (forall x, x <= Z.of_nat N -> 0 <= f x)
+-> (forall (m : nat), (m <= n)%nat -> f (Z.of_nat m) <= total).
+Proof.
+  intros f total n N HtotalBalance HnLeN Hfnneg m HmLen .
+  assert (0 <= total) as HtotalNneg. { 
+    rewrite <- HtotalBalance. apply sum_pos with (N := N); [assumption | lia].
+  }
+
+  assert (forall x acc, f (Z.of_nat (S x)) = balanceOf_sum' f (S x) acc - balanceOf_sum' f x acc). {
+    intros. simpl. rewrite balanceOf_sum_acc. lia. 
+  }
+  assert (f 0 = balanceOf_sum' f 0 0). { simpl; lia. }
+
+  destruct m.
+  - rewrite <- HtotalBalance. rewrite Nat2Z.inj_0. rewrite H0.
+    apply sum_mono.
+    + intros. apply Hfnneg with (x := Z.of_nat x). lia.
+    + lia.
+  - rewrite H with (acc := 0).
+    rewrite <- HtotalBalance.
+    rewrite <- Z.sub_0_r with (n := balanceOf_sum' f N 0).
+    apply Z.sub_le_mono.
+    + apply sum_mono.
+      * intros. apply Hfnneg with (x := Z.of_nat x). lia.
+      * lia.
+    + apply sum_pos with (N := N).
+      * intros. apply Hfnneg. lia.
+      * lia.
+Qed.
+
+Definition Amm_balance_nneg_Prop (ENV : Env) (T0 T1 : Token.State) (L : Z) (NextAddr : address) (STATE : State) : Prop :=
+  forall x, 0 <= balanceOf STATE x.
+
+Lemma Amm_balance_nneg_init : invariantInit Amm_balance_nneg_Prop.
+Proof.
+  unfold invariantInit, Amm_balance_nneg_Prop.
+  intros.
+  destruct H.
+  simpl.
+  destruct (x =? Caller ENV) eqn:Hcond1.
+  - destruct (x =? This ENV) eqn:Hcond2.
+    + lia.
+    + destruct H_conds; lia.
+  - destruct (x =? This ENV) eqn:Hcond2; lia.
+Qed.
+
+Lemma Amm_balance_nneg_step : invariantStep Amm_balance_nneg_Prop.
+Proof.
+  unfold invariantStep, Amm_balance_nneg_Prop.
+  intros ENV0 t0 t1 liquidity NextAddr0 STATE STATE' H_conds0 Hstep Hyp x.
+  destruct Hstep as [ENV [NextAddr [NextAddr' Htransition]]].
+  destruct Htransition
+    as [ HAmmStep
+       | _ _ Hcaller_cnstr _ HTokenTransition Haddr_const _ _ Hbalance_const _ _ Htk1_const
+       | _ _ Hcaller_cnstr _ HTokenTransition Haddr_const _ _ Hbalance_const _ _ Htk0_const].
+  - destruct HAmmStep; simpl; auto;
+    destruct H; simpl; destruct H_conds; destruct_ifs; try apply Hyp; try lia.
+  - destruct HTokenTransition. rewrite <- Hbalance_const. apply Hyp.
+  - destruct HTokenTransition. rewrite <- Hbalance_const. apply Hyp.
+Qed.
+
+Lemma Amm_balance_nneg_reach : 
+  forall (ENV : Env) (t0 : Token.State) (t1 : Token.State) (liquidity : Z) (NextAddr : address) (STATE : State),
+     reachableFromInit ENV t0 t1 liquidity (NextAddr : address) (STATE : State)
+  -> Amm_balance_nneg_Prop ENV t0 t1 liquidity NextAddr STATE
+.
+Proof.
+  intros.
+  apply invariantReachable.
+  exact Amm_balance_nneg_init.
+  exact Amm_balance_nneg_step.
+  assumption.
+Qed.
+
+Definition Amm_reserve_nneg_Prop (ENV : Env) (T0 T1 : Token.State) (L : Z) (NextAddr : address) (STATE : State) : Prop :=
+  0 <= reserve0 STATE /\ 0 <= reserve1 STATE.
+
+Lemma Amm_reserve_nneg_init : invariantInit Amm_reserve_nneg_Prop.
+Proof.
+  unfold invariantInit, Amm_reserve_nneg_Prop.
+  intros.
+  destruct H; destruct H_conds.
+  simpl.
+  split; lia.
+Qed.
+
+Lemma Amm_reserve_nneg_step : invariantStep Amm_reserve_nneg_Prop.
+Proof.
+  unfold invariantStep, Amm_reserve_nneg_Prop.
+  intros ENV0 t0 t1 liquidity NextAddr0 STATE STATE' HinitPrecs Hstep Hyp.
+  destruct Hstep as [ENV [NextAddr [NextAddr' Htransition]]].
+  destruct Htransition
+    as [ HAmmStep
+       | _ _ Hcaller_cnstr _ HTokenTransition Haddr_const _ _ Hbalance_const Hres0_const Hres1_const Htk1_const
+       | _ _ Hcaller_cnstr _ HTokenTransition Haddr_const _ _ Hbalance_const Hres0_const Hres1_const Htk0_const].
+  - destruct HAmmStep; simpl; auto;
+    destruct H; destruct H_conds; simpl; lia.
+  - destruct HTokenTransition. rewrite <- Hres0_const, <- Hres1_const. apply Hyp.
+  - destruct HTokenTransition. rewrite <- Hres0_const, <- Hres1_const. apply Hyp.
+Qed.
+
+Lemma Amm_reserve_nneg_reach : 
+  forall (ENV : Env) (t0 : Token.State) (t1 : Token.State) (liquidity : Z) (NextAddr : address) (STATE : State),
+     reachableFromInit ENV t0 t1 liquidity NextAddr (STATE : State)
+  -> Amm_reserve_nneg_Prop ENV t0 t1 liquidity NextAddr STATE
+.
+Proof.
+  intros.
+  apply invariantReachable.
+  exact Amm_reserve_nneg_init.
+  exact Amm_reserve_nneg_step.
+  assumption.
+Qed.
+
+Definition Amm_solvency_Prop (ENV : Env) (T0 T1 : Token.State) (L : Z) (STATE : State) : Prop :=
+  forall x, 0 <= x <= MAX_ADDRESS ->
+  0 < balanceOf STATE x ->
+  balanceOf STATE x * reserve0 STATE / totalSupply STATE <= Token.balanceOf (token0 STATE) (addr STATE) /\
+  balanceOf STATE x * reserve1 STATE / totalSupply STATE <= Token.balanceOf (token1 STATE) (addr STATE).
+
+Lemma Amm_solvency_reach : 
+  forall (ENV : Env) (t0 : Token.State) (t1 : Token.State) (liquidity : Z) (NextAddr : address) (STATE : State),
+     reachableFromInit ENV t0 t1 liquidity NextAddr STATE
+     (*-> totalSupply STATE  > 0*)
+  -> Amm_solvency_Prop ENV t0 t1 liquidity STATE
+.
+Proof.
+  intros.
+  assert (Amm_liqs_sum_eq_total_AssistedProp ENV t0 t1 liquidity NextAddr STATE) as HsumEq. {
+    apply Amm_liqs_sum_eq_total_reach. assumption.
+  }
+  assert (Amm_balance_nneg_Prop ENV t0 t1 liquidity NextAddr STATE) as HbalNneg. {
+    apply Amm_balance_nneg_reach. assumption.
+  }
+  assert (Amm_reserve_nneg_Prop ENV t0 t1 liquidity NextAddr STATE) as [Hres0Nneg Hres1Nneg]. {
+    apply Amm_reserve_nneg_reach. assumption.
+  }
+  unfold Amm_solvency_Prop.
+  unfold Amm_liqs_sum_eq_total_AssistedProp in HsumEq.
+  intros.
+
+  assert (forall p, 0 <= p <= MAX_ADDRESS -> balanceOf STATE p <= totalSupply STATE) as HbalLeTotal. {
+    intros.
+    unfold Amm_liqs_sum_eq_total_Prop in HsumEq.
+    destruct HsumEq as [_ [_ [_ [ _ H']]]].
+    (*rewrite <- H'.*)
+    remember (Z.to_nat p) as pn eqn:Heqpn.
+    assert (p = Z.of_nat pn) as Heqp. { rewrite Heqpn. apply Z.eq_sym_iff. apply Z2Nat.id. lia. }
+    rewrite Heqp.
+    apply sum_le_total' with (f := balanceOf STATE) (total := totalSupply STATE) (n := pn) (N := Z.to_nat MAX_ADDRESS).
+    - assumption.
+    - lia.
+    - intros. apply HbalNneg.
+    - lia.
+    }
+  assert (0 < totalSupply STATE). {
+    apply Z.lt_le_trans with (m := balanceOf STATE x).
+    - assumption.
+    - apply HbalLeTotal. assumption.
+  }
+  split.
+  - apply Z.le_trans with (m := totalSupply STATE * reserve0 STATE / totalSupply  STATE).
+    + apply Z.div_le_mono.
+      * lia.
+      * apply Z.mul_le_mono_nonneg_r.
+        -- assumption.
+        -- apply HbalLeTotal. lia.
+    + rewrite Z.mul_comm, Z.div_mul. destruct HsumEq as [_ [_ [H' [_ _]]]].
+      apply H'.
+      lia.
+  - apply Z.le_trans with (m := totalSupply STATE * reserve1 STATE / totalSupply  STATE).
+    + apply Z.div_le_mono.
+      * lia.
+      * apply Z.mul_le_mono_nonneg_r.
+        -- assumption.
+        -- apply HbalLeTotal. lia.
+    + rewrite Z.mul_comm, Z.div_mul. destruct HsumEq as [_ [_ [_ [H' _]]]].
+      apply H'.
+      lia.
+Qed.
