tests/rocq/ERC20/Theory.v
@@ -10,8 +10,24 @@ Import Token.
 
 (* Address should be Z or N? Or int20? *)
 
-Definition MAX_ADDRESS := UINT_MAX 160.
+Ltac destructAnds :=
+  repeat match goal with
+    [ H : _ /\ _ |- _ ] => destruct H
+  end.
 
+Ltac rewrite_eqbs :=
+  repeat match goal with
+  | [ H : ?a = ?b |- context [?a =? ?b] ] =>
+    rewrite (proj2 (Z.eqb_eq a b) H)
+  | [ H : ?a = ?b |- context [?b =? ?a] ] =>
+    rewrite (proj2 (Z.eqb_eq b a) (eq_sym H))
+  | [ H : ?a <> ?b |- context [?a =? ?b] ] =>
+    rewrite (proj2 (Z.eqb_neq a b) H)
+  | [ H : ?a <> ?b |- context [?b =? ?a] ] =>
+    rewrite (proj2 (Z.eqb_neq b a) (not_eq_sym H))
+  end.
+
+Definition MAX_ADDRESS := UINT_MAX 160.
 
 Fixpoint balanceOf_sum' (balanceOf : address -> Z) (n : nat) (acc : Z) : Z :=
     match n with
@@ -33,46 +49,6 @@ Definition transfer map from to amt := transfer_to (transfer_from map from amt) 
 
 Definition transfer' map from to amt := transfer_from (transfer_to map to amt) from amt.
 
-Inductive transferRelation from to amt (map : address -> Z) (map' : address -> Z) : Prop:= 
-  | transferEqC:
-      from <> to
-  -> (forall p, p <> from -> p <> to -> map p = map' p)
-  -> map from = map' from + amt 
-  -> map to + amt= map' to
-  -> transferRelation from to amt map map'
-  | transferNeqC:
-      from = to
-  -> (forall p, map p = map' p)
-  -> transferRelation from to amt map map'.
-
-Inductive transferStateRelation from to amt s s' : Prop:= 
-  | transferStateC: 
-    transferRelation from to amt (balanceOf s) (balanceOf s')
-    -> transferStateRelation from to amt s s'.
-
-Inductive mintRelation to amt map (map' : address -> Z) : Prop:= 
-  | mintC: 
-  map to + amt= map' to
-  -> (forall p, p <> to -> map p = map' p)
-  ->  mintRelation to amt map map'.
-
-Inductive mintStateRelation to amt s s' : Prop:= 
-  | mintStateC: 
-    mintRelation to amt (balanceOf s) (balanceOf s')
-    -> mintStateRelation to amt s s'.
-
-Inductive burnRelation from amt map (map' : address -> Z) : Prop:= 
-  | burnC: 
-      map from = map' from + amt
-  -> (forall p, p <> from -> map p = map' p)
-  ->  burnRelation from amt map map'.
-
-Inductive burnStateRelation from amt s s' : Prop:= 
-  | burnStateC: 
-    burnRelation from amt (balanceOf s) (balanceOf s')
-    -> burnStateRelation from amt s s'.
-
-
 Lemma balanceOf_sum_f_eq f f' addr acc :
   (forall x, x <= Z.of_nat addr -> f x = f' x) ->
   balanceOf_sum' f addr acc = balanceOf_sum' f' addr acc.
@@ -92,7 +68,6 @@ Proof.
 Qed.
 
 Opaque Z.sub Z.add Z.of_nat.
-
 
 Lemma balanceOf_sum_thm x f f' addr acc :
   (forall y, x <> y -> f y = f' y) ->
@@ -133,191 +108,48 @@ Proof.
         intros Heq; subst. lia.
 Qed.
 
-
-Lemma balanceOf_sum_transfer_from map from amt addr acc :
-  0 <= from ->
-  balanceOf_sum' (transfer_from map from amt) addr acc =
-  if (Z.to_nat from <=? addr)%nat then balanceOf_sum' map addr acc - amt else balanceOf_sum' map addr acc.
+Lemma balanceOf_sum_thm' x f f' acc :
+  (forall y, x <> y -> f y = f' y) ->
+  0 <= x <= MAX_ADDRESS->
+  balanceOf_sum' f (Z.to_nat MAX_ADDRESS) acc = balanceOf_sum' f' (Z.to_nat MAX_ADDRESS) acc - f' x + f x.
 Proof.
-  intros Hleq1.
-  erewrite balanceOf_sum_thm with (f := transfer_from map from amt) (f' := map) (x := from); eauto.
-
-  - destruct (Z.to_nat from <=? addr)%nat eqn:Hleq.
-
-    unfold transfer_from. rewrite Z.eqb_refl. lia.
-
+  intros H_f [H_x_0 H_x_max].
+  rewrite balanceOf_sum_thm with (x := x) (f' := f').
+  - apply Z2Nat.inj_le in H_x_max; try lia.
+    rewrite <- Nat.leb_le in H_x_max.
+    rewrite H_x_max.
     reflexivity.
-
-  - intros. unfold transfer_from. eapply Z.eqb_neq in H.
-    rewrite Z.eqb_sym, H. reflexivity.
+  - assumption.
+  - assumption.
 Qed.
 
-Lemma balanceOf_sum_burnFrom map from amt addr acc map' :
-  0 <= from ->
-  burnRelation from amt map map' ->
-  balanceOf_sum' map' addr acc =
-  if (Z.to_nat from <=? addr)%nat then balanceOf_sum' map addr acc - amt else balanceOf_sum' map addr acc.
+Lemma balanceOf_sum_transfer_thm x1 x2 f f' acc :
+  (forall y, x1 <> y -> x2 <> y -> f y = f' y) ->
+  f x1 + f x2 = f' x1 + f' x2 ->
+  0 <= x1 <= MAX_ADDRESS ->
+  0 <= x2 <= MAX_ADDRESS ->
+  balanceOf_sum' f (Z.to_nat MAX_ADDRESS) acc = balanceOf_sum' f' (Z.to_nat MAX_ADDRESS) acc.
 Proof.
-  intros Hleq1 Hburn.
-  destruct Hburn as [HburnFrom HburnElse].
-  erewrite balanceOf_sum_thm with (f := map') (f' := map) (x := from); eauto.
-
-  - destruct (Z.to_nat from <=? addr)%nat eqn:Hleq.
-    lia. lia.
-
-  - intros. rewrite Z.eq_sym_iff. apply HburnElse. lia.
-Qed.
-
-Lemma balanceOf_sum_mintTo map to amt addr acc map':
-  0 <= to ->
-  mintRelation to amt map map' ->
-  balanceOf_sum' map' addr acc =
-  if (Z.to_nat to <=? addr)%nat then balanceOf_sum' map addr acc + amt else balanceOf_sum' map addr acc.
-Proof.
-  intros Hleq1 Hmint.
-  destruct Hmint as [HmintFrom HmintElse].
-  erewrite balanceOf_sum_thm with (f := map') (f' := map) (x := to); eauto.
-
-  - destruct (Z.to_nat to <=? addr)%nat eqn:Hleq.
-    lia. lia.
-
-  - intros. rewrite Z.eq_sym_iff. apply HmintElse. lia.
-Qed.
-
-Ltac convert_neq :=
-  repeat match goal with
-    [ H : _ <> _ |- _ ] => let H_og := fresh H "'" in eapply not_eq_sym in H as H_og; eapply Z.eqb_neq in H; eapply Z.eqb_neq in H_og
-  end.
-
-Ltac convert_eq :=
-  repeat match goal with
-    [ H : _ = _ |- _ ] => let H_og := fresh H "'" in eapply eq_sym in H as H_og; eapply Z.eqb_eq in H; eapply Z.eqb_eq in H_og
-  end.
-
-Ltac destructAnds :=
-  repeat match goal with
-    [ H : _ /\ _ |- _ ] => destruct H
-  end.
-
-Ltac rewrite_eqs :=
-  repeat match goal with
-    [ H : _ =? _ = _ |- _ ] => rewrite H
-  end.
-
-Theorem transfer_burn_mint from to amt map imap map':
-  0 <= from ->
-  0 <= to ->
-  transferRelation from to amt map map' ->
-  imap = (fun p => if p =? from then map p - amt else map p) ->
-  (burnRelation from amt map imap
-  /\ mintRelation to amt imap map').
-Proof.
-  intros Hleq1 Hleq2 Htransfer Himap.
-  rewrite Himap in *.
-  split.
-  - constructor.
-    + rewrite Z.eqb_refl. lia.
-    + destruct Htransfer; intros p Hpleq; convert_neq; rewrite_eqs; reflexivity.
-  - constructor.
-    + destruct Htransfer.
-      * convert_neq. rewrite_eqs. assumption.
-      * convert_eq. rewrite_eqs. rewrite H0. lia.
-    + destruct Htransfer; intros p Hpneq.
-      * destruct (p =? from) eqn:HpFrom.
-        -- apply Z.eqb_eq in HpFrom. rewrite HpFrom. lia.
-        -- apply H0; [apply Z.eqb_neq| ]; assumption.
-      * convert_neq. rewrite H. rewrite_eqs. rewrite H0. lia.
-Qed.
-
-
-Theorem transfer_thm map from to amt addr acc: forall map',
-  to <> from ->
-  0 <= from <= Z.of_nat addr ->
-  0 <= to <= Z.of_nat addr ->
-  transferRelation from to amt map map' ->
-  balanceOf_sum' map' addr acc  = balanceOf_sum' map addr acc.
-Proof.
-  intros map' Hneq Hleq1 Hleq2 Htransfer.
-  eapply transfer_burn_mint in Htransfer.
-  4: constructor.
-  remember (fun p : Z => if p =? from then map p - amt else map p) as imap.
-  destruct Htransfer.
-  - rewrite balanceOf_sum_mintTo with (map' := map') (map := imap) (to := to) (amt := amt); [ | lia | assumption ].
-    + rewrite leb_correct; [ | lia];
-      rewrite balanceOf_sum_burnFrom with (map' := imap) (map := map) (from := from) (amt := amt).
-        -- rewrite leb_correct; lia.
-        -- lia.
-        -- assumption.
+  intros H_f1 H_f2 [H_x1_0 H_x1_max] [H_x2_0 H_x2_max].
+  rewrite balanceOf_sum_thm with (x := x1) (f' := fun _b => if _b =? x1 then f' _b else f _b).
+  - apply Z2Nat.inj_le in H_x1_max; try lia.
+    rewrite <- Nat.leb_le in H_x1_max.
+    rewrite H_x1_max, Z.eqb_refl.
+    rewrite balanceOf_sum_thm with (x := x2) (f' := f').
+    + apply Z2Nat.inj_le in H_x2_max; try lia.
+      rewrite <- Nat.leb_le in H_x2_max.
+      rewrite H_x2_max.
+      destruct (x2 =? x1) eqn:Hx2x1.
+      * apply Z.eqb_eq in Hx2x1. subst. lia.
+      * lia.
+    + intros. destruct (y =? x1) eqn:Hyx1.
+      * lia.
+      * apply H_f1; [lia | assumption].
+    + lia.
+  - intros. destruct (y =? x1) eqn:Hyx1.
+    * apply H_f1; [assumption | lia].
+    * reflexivity.
   - lia.
-  - lia.
-Qed.
-
-Lemma balances_after_transfer STATE src dst amount STATE' :
-  0 <= src <= MAX_ADDRESS ->
-  0 <= dst <= MAX_ADDRESS ->
-  src <> dst ->
-  transferStateRelation src dst amount STATE STATE' ->
-  balanceOf_sum STATE = balanceOf_sum STATE' .
-Proof.
-  intros. unfold balanceOf_sum; simpl.
-  apply Z.eq_sym_iff.
-  apply transfer_thm with (from := src) (to := dst) (amt := amount).
-
-  + lia.
-  + lia.
-  + lia.
-  + destruct H2.
-    assumption.
-Qed.
-
-Lemma balances_after_burn STATE src  amount STATE' :
-  0 <= src <= MAX_ADDRESS ->
-  burnStateRelation src amount STATE STATE' ->
-  balanceOf_sum STATE - amount =
-  balanceOf_sum STATE'.
-Proof.
-  intros. unfold balanceOf_sum; simpl.
-
-  assert (forall map amt addr acc map', src <= addr ->
-    burnRelation src amt map map' ->
-    balanceOf_sum' map' (Z.to_nat addr) acc =
-    balanceOf_sum' map (Z.to_nat addr) acc - amt) as HburnFrom.
-  { intros. rewrite balanceOf_sum_burnFrom with (map := map) (from := src) (amt := amt); [ | lia | assumption ].
-
-    destruct (Z.to_nat src <=? Z.to_nat addr0)%nat eqn:Hleq.
-    + reflexivity.
-    + apply Nat.leb_nle in Hleq. lia.
-  }
-
-  rewrite Z.eq_sym_iff.
-  apply HburnFrom; [lia | ].
-  destruct H0.
-  assumption.
-Qed.
-
-Lemma balances_after_mint STATE dst amount STATE':
-  0 <= dst <= MAX_ADDRESS ->
-  mintStateRelation dst amount STATE STATE' ->
-  balanceOf_sum STATE + amount =
-  balanceOf_sum STATE'.
-Proof.
-  intros. unfold balanceOf_sum; simpl.
-
-  assert (forall map amt addr acc map', dst <= addr ->
-  mintRelation dst amt map map' ->
-  balanceOf_sum' map' (Z.to_nat addr) acc =
-  balanceOf_sum' map (Z.to_nat addr) acc + amt) as HmintTo.
-  { intros. rewrite balanceOf_sum_mintTo with (map := map) (to := dst) (amt := amt); [ | lia | assumption ].
-
-    destruct (Z.to_nat dst <=? Z.to_nat addr0)%nat eqn:Hleq.
-    + reflexivity.
-    + apply Nat.leb_nle in Hleq. lia.
-  }
-
-  rewrite Z.eq_sym_iff.
-  apply HmintTo; [lia | ].
-  destruct H0.
-  assumption.
 Qed.
 
 Theorem initialSupply': forall ENV _totalSupply (n : nat), forall NA NA' STATE,
@@ -413,142 +245,54 @@ Proof.
     assert ( forall a b c,
       a - b = -c <-> a + c = b) as Ha4. lia.
 
-    destruct Hstep as [ENV [NA [NA' Hextstep]]].
-    destruct Hextstep as [Hstep].
+    destruct Hstep as [ENV [NA [NA' Htransition]]].
+    destruct Htransition as [Hstep].
     destruct Hstep.
-    + remember STATE' eqn:Hstate'.
-      destruct H.
-      * apply deltas with (x1 := balanceOf_sum STATE) (y1 := totalSupply STATE); [ assumption | simpl; destruct H_conds ].
-        simpl.
-        rewrite Hstate'. unfold MAX_ADDRESS in *.
-        rewrite Z.sub_diag with (n := totalSupply STATE);
-        apply Zeq_minus;
-        eapply (balances_after_transfer) with (src := Caller ENV) (dst := to) (amount := _value); [ | |simpl |]. try split; unfold MAX_ADDRESS; try split; try lia. unfold MAX_ADDRESS. lia. lia.
-        constructor.
-        {
-          constructor.
-          - lia.
-          - intros p Hneq1 Hneq2.
-            rewrite <- Hstate'.
-            simpl. convert_neq. rewrite_eqs. reflexivity.
-          - rewrite <- Hstate'.
-            simpl. convert_neq. rewrite_eqs. rewrite Z.eqb_refl. lia.
-          - rewrite <- Hstate'.
-            simpl. convert_neq. rewrite_eqs. rewrite Z.eqb_refl. lia.
-            }
-      * simpl. rewrite <- IHHmulti. reflexivity.
-    + remember STATE' eqn:Hstate'.
-      destruct H.
-      * apply deltas with (x1 := balanceOf_sum STATE) (y1 := totalSupply STATE); [ assumption | simpl; destruct H_conds ].
-        simpl.
-        rewrite Hstate'. unfold MAX_ADDRESS in *.
-        rewrite Z.sub_diag with (n := totalSupply STATE);
-        apply Zeq_minus;
-        eapply (balances_after_transfer) with (src := src) (dst := dst) (amount := amount); [ | |simpl |]. try split; unfold MAX_ADDRESS; try split; try lia. unfold MAX_ADDRESS. lia. lia.
-        constructor.
-        {
-          constructor.
-          - lia.
-          - intros p Hneq1 Hneq2.
-            rewrite <- Hstate'.
-            simpl. convert_neq. rewrite_eqs. reflexivity.
-          - rewrite <- Hstate'.
-            simpl. convert_neq. rewrite_eqs. rewrite Z.eqb_refl. lia.
-          - rewrite <- Hstate'. destruct H_case_cond.
-            simpl. convert_neq. rewrite_eqs. rewrite Z.eqb_refl. lia.
-            }
-      * apply deltas with (x1 := balanceOf_sum STATE) (y1 := totalSupply STATE); [ assumption | simpl; destruct H_conds ].
-        simpl.
-        rewrite Hstate'. unfold MAX_ADDRESS in *.
-        rewrite Z.sub_diag with (n := totalSupply STATE);
-        apply Zeq_minus;
-        eapply (balances_after_transfer) with (src := src) (dst := dst) (amount := amount); [ | |simpl |]. try split; unfold MAX_ADDRESS; try split; try lia. unfold MAX_ADDRESS. lia. lia.
-        constructor.
-        {
-          constructor.
-          - lia.
-          - intros p Hneq1 Hneq2.
-            rewrite <- Hstate'.
-            simpl. convert_neq. rewrite_eqs. reflexivity.
-          - rewrite <- Hstate'.
-            simpl. convert_neq. rewrite_eqs. rewrite Z.eqb_refl. lia.
-          - rewrite <- Hstate'. destruct H_case_cond. destruct H.
-            simpl. convert_neq. rewrite_eqs. rewrite Z.eqb_refl. lia.
-            }
-      * apply deltas with (x1 := balanceOf_sum STATE) (y1 := totalSupply STATE); [ assumption | simpl; destruct H_conds ].
-        simpl.
-        rewrite Hstate'. unfold MAX_ADDRESS in *.
-        rewrite Z.sub_diag with (n := totalSupply STATE);
-        apply Zeq_minus;
-        eapply (balances_after_transfer) with (src := src) (dst := dst) (amount := amount); [ | |simpl |]. try split; unfold MAX_ADDRESS; try split; try lia. unfold MAX_ADDRESS. lia. lia.
-        constructor.
-        {
-          constructor.
-          - lia.
-          - intros p Hneq1 Hneq2.
-            rewrite <- Hstate'.
-            simpl. convert_neq. rewrite_eqs. reflexivity.
-          - rewrite <- Hstate'.
-            simpl. convert_neq. rewrite_eqs. rewrite Z.eqb_refl. lia.
-          - rewrite <- Hstate'. destruct H_case_cond. destruct H.
-            simpl. convert_neq. rewrite_eqs. rewrite Z.eqb_refl. lia.
-            }
-      * simpl. rewrite <- IHHmulti at 2. reflexivity.
-      * simpl. rewrite <- IHHmulti at 2. reflexivity.
-    + destruct H; simpl; rewrite <- IHHmulti; unfold balanceOf_sum;  simpl; reflexivity.
-    + remember STATE' eqn:Hstate'.
-      destruct H.
-      * apply deltas with (x1 := balanceOf_sum STATE) (y1 := totalSupply STATE); [ assumption | simpl; destruct H_conds ].
-        simpl.
-        rewrite Hstate'. unfold MAX_ADDRESS in *.
-        rewrite Ha1. rewrite Ha2.
-        eapply (balances_after_burn) with (src := Caller ENV) (amount := amount); [ unfold MAX_ADDRESS; split; lia | simpl ].
-        constructor.
-        constructor.
-        -- rewrite <- Hstate'; simpl. rewrite Z.eqb_refl. lia.
-        -- intros p Hneq.
-           rewrite <- Hstate'; simpl. convert_neq. rewrite_eqs. lia.
-    + remember STATE' eqn:Hstate'.
-      destruct H.
-      * apply deltas with (x1 := balanceOf_sum STATE) (y1 := totalSupply STATE); [ assumption | simpl; destruct H_conds ].
-        rewrite Hstate'.
-        rewrite Ha1. rewrite Ha2.
-        eapply (balances_after_burn) with (src := src) (amount := amount); [ unfold MAX_ADDRESS; split; lia | simpl ].
-        constructor.
-        constructor.
-        -- rewrite <- Hstate'; simpl. rewrite Z.eqb_refl. lia.
-        -- intros p Hneq.
-           rewrite <- Hstate'; simpl. convert_neq. rewrite_eqs. lia.
-      * apply deltas with (x1 := balanceOf_sum STATE) (y1 := totalSupply STATE); [ assumption | simpl; destruct H_conds].
-        rewrite Hstate'.
-        rewrite Ha1. rewrite Ha2.
-        eapply (balances_after_burn) with (src := src) (amount := amount); [ unfold MAX_ADDRESS; split; lia | simpl ].
-        constructor.
-        constructor.
-        -- rewrite <- Hstate'; simpl. rewrite Z.eqb_refl. lia.
-        -- intros p Hneq.
-           rewrite <- Hstate'; simpl. convert_neq. rewrite_eqs. lia.
-      * apply deltas with (x1 := balanceOf_sum STATE) (y1 := totalSupply STATE); [ assumption | simpl; destruct H_conds ].
-        rewrite Hstate'.
-        rewrite Ha1. rewrite Ha2.
-        eapply (balances_after_burn) with (src := src) (amount := amount); [ unfold MAX_ADDRESS; split; lia | simpl ].
-        constructor.
-        constructor.
-        -- rewrite <- Hstate'; simpl. rewrite Z.eqb_refl. lia.
-        -- intros p Hneq.
-           rewrite <- Hstate'; simpl. convert_neq. rewrite_eqs. lia.
-    + remember STATE' eqn:Hstate'.
-      destruct H.
-      * apply deltas with (x1 := balanceOf_sum STATE) (y1 := totalSupply STATE); [ assumption | simpl; destruct H_conds ].
-        rewrite Hstate'.
-        rewrite Ha3. rewrite Ha4.
-        eapply (balances_after_mint) with (dst := dst) (amount := amount); [ unfold MAX_ADDRESS; split; lia | simpl ].
-        constructor.
-        constructor.
-        -- rewrite <- Hstate'; simpl. rewrite Z.eqb_refl. lia.
-        -- intros p Hneq.
-           rewrite <- Hstate'; simpl. convert_neq. rewrite_eqs. lia.
-    + destruct H. simpl. unfold balanceOf_sum. rewrite <- IHHmulti.  simpl; reflexivity.
-    + destruct H. simpl. unfold balanceOf_sum. rewrite <- IHHmulti.  simpl; reflexivity.
-    + destruct H. simpl. unfold balanceOf_sum. rewrite <- IHHmulti.  simpl; reflexivity.
+    + (* transfer *)
+      apply deltas with (x1 := balanceOf_sum STATE) (y1 := totalSupply STATE); [assumption|].
+      unfold balanceOf_sum.
+      rewrite balanceOf_sum_transfer_thm with (x1 := Caller ENV) (x2 := to) (f' := balanceOf STATE').
+      * destruct H; simpl; lia.
+      * destruct H; simpl; intros; rewrite_eqbs; reflexivity.
+      * destruct H; simpl; rewrite_eqbs; repeat rewrite Z.eqb_refl; lia.
+      * destruct H; simpl; unfold MAX_ADDRESS; destruct H_conds; lia.
+      * destruct H; simpl; unfold MAX_ADDRESS; destruct H_conds; lia.
+    + (* transferFrom *)
+      apply deltas with (x1 := balanceOf_sum STATE) (y1 := totalSupply STATE); [assumption|].
+      unfold balanceOf_sum. simpl.
+      rewrite balanceOf_sum_transfer_thm with (x1 := src) (x2 := dst) (f' := balanceOf STATE').
+      * destruct H; simpl; lia.
+      * destruct H; simpl; intros; rewrite_eqbs; reflexivity.
+      * destruct H; simpl; destructAnds; rewrite_eqbs; repeat rewrite Z.eqb_refl; lia.
+      * destruct H; simpl; unfold MAX_ADDRESS; destruct H_conds; lia.
+      * destruct H; simpl; unfold MAX_ADDRESS; destruct H_conds; lia.
+    + (* approve *)
+      destruct H; simpl; auto.
+    + (* burn *)
+      apply deltas with (x1 := balanceOf_sum STATE) (y1 := totalSupply STATE); [assumption|].
+      unfold balanceOf_sum. simpl.
+      rewrite balanceOf_sum_thm' with (x := Caller ENV) (f' := balanceOf STATE').
+      * destruct H; simpl; rewrite Z.eqb_refl; lia.
+      * destruct H; simpl; intros; rewrite_eqbs; reflexivity.
+      * destruct H; simpl; unfold MAX_ADDRESS; destruct H_conds; lia.
+    + (* burnFrom *)
+      apply deltas with (x1 := balanceOf_sum STATE) (y1 := totalSupply STATE); [assumption|].
+      unfold balanceOf_sum. simpl.
+      rewrite balanceOf_sum_thm' with (x := src) (f' := balanceOf STATE').
+      * destruct H; simpl; rewrite Z.eqb_refl; lia.
+      * destruct H; simpl; intros; rewrite_eqbs; reflexivity.
+      * destruct H; simpl; unfold MAX_ADDRESS; destruct H_conds; lia.
+    + (* mint *)
+      apply deltas with (x1 := balanceOf_sum STATE) (y1 := totalSupply STATE); [assumption|].
+      unfold balanceOf_sum. simpl.
+      rewrite balanceOf_sum_thm' with (x := dst) (f' := balanceOf STATE').
+      * destruct H; simpl; rewrite Z.eqb_refl; lia.
+      * destruct H; simpl; intros; rewrite_eqbs; reflexivity.
+      * destruct H; simpl; unfold MAX_ADDRESS; destruct H_conds; lia.
+    + (* totalSupply *)
+      destruct H; simpl; auto.
+    + (* balanceOf *)
+      destruct H; simpl; auto.
+    + (* allowance *)
+      destruct H; simpl; auto.
 Qed.
